Setup structure for proof of Loop elimination

pancake/proofs/wheat_loopProofScript.sml
@@ -18,8 +18,8 @@ Definition every_prog_def:
     p (If x1 x2 x3 p1 p2 l1) /\ every_prog p p1 /\ every_prog p p2) /\
   (every_prog p (Mark p1) <=>
     p (Mark p1) /\ every_prog p p1) /\
-  (every_prog p (Call ret dest args handler) <=>
-    p (Call ret dest args handler) /\
+  (every_prog p (Call ret dest args handler l) <=>
+    p (Call ret dest args handler l) /\
     (case handler of SOME (n,q) => every_prog p q | NONE => T)) /\
   (every_prog p prog <=> p prog)
 End
@@ -28,19 +28,18 @@ Definition no_Loop_def:
   no_Loop = every_prog (\q. !l1 x l2. q <> Loop l1 x l2)
 End
 
-Definition comp_no_loop_def:
-  (comp_no_loop p (Seq p1 p2) =
-    Seq (comp_no_loop p p1) (comp_no_loop p p2)) /\
-  (comp_no_loop p (If x1 x2 x3 p1 p2 l1) =
-    If x1 x2 x3 (comp_no_loop p p1) (comp_no_loop p p2) l1) /\
-  (comp_no_loop p (Call ret dest args handler) =
-    Call ret dest args (case handler of
-                        | SOME (n,q) => SOME (n,comp_no_loop p q)
-                        | NONE => NONE)) /\
-  (comp_no_loop p Break = FST p) /\
-  (comp_no_loop p Continue = SND p) /\
-  (comp_no_loop p (Mark prog) = comp_no_loop p prog) /\
-  (comp_no_loop p prog = prog)
+Definition syntax_ok_def:
+  (syntax_ok (Seq p1 p2) <=>
+    ~(no_Loop (Seq p1 p2)) ∧ syntax_ok p1 /\ syntax_ok p2) /\
+  (syntax_ok (Loop l1 body l2) <=>
+    syntax_ok body) /\
+  (syntax_ok (If x1 x2 x3 p1 p2 l1) <=>
+    ~(no_Loop (If x1 x2 x3 p1 p2 l1)) ∧ syntax_ok p1 /\ syntax_ok p2) /\
+  (syntax_ok (Mark p1) <=>
+    no_Loop p1) /\
+  (syntax_ok (Call ret dest args handler l) <=>
+    (case handler of SOME (n,q) => syntax_ok q | NONE => F)) /\
+  (syntax_ok prog <=> F)
 End
 
 Definition mark_all_def:
@@ -59,63 +58,306 @@ Definition mark_all_def:
      let t3 = (t1 /\ t2) in
        (if t3 then Mark p3 else p3, t3)) /\
   (mark_all (Mark p1) = mark_all p1) /\
-  (mark_all (Call ret dest args handler) =
+  (mark_all (Call ret dest args handler l) =
      case handler of
-     | NONE => (Mark (Call ret dest args handler), T)
+     | NONE => (Mark (Call ret dest args handler l), T)
      | SOME (n,p1) =>
          let (p1,t1) = mark_all p1 in
-         let p2 = Call ret dest args (SOME (n,p1)) in
+         let p2 = Call ret dest args (SOME (n,p1)) l in
            (if t1 then Mark p2 else p2, t1)) /\
   (mark_all prog = (Mark prog,T))
 End
 
-Theorem mark_all_correct:
-  !prog q b.
-     mark_all prog = (q,b) ==>
-     b = no_Loop q /\
-     every_prog (\p. !q. p = Mark q ==> no_Loop q) q
+Theorem evaluate_Loop_body_same:
+  (∀(s:('a,'b)state). evaluate (body,s) = evaluate (body',s)) ⇒
+  ∀(s:('a,'b)state). evaluate (Loop l1 body l2,s) = evaluate (Loop l1 body' l2,s)
 Proof
-  recInduct mark_all_ind \\ reverse (rpt conj_tac)
+  rw [] \\ completeInduct_on ‘s.clock’
+  \\ rw [] \\ fs [PULL_EXISTS,PULL_FORALL]
+  \\ once_rewrite_tac [evaluate_def]
+  \\ CASE_TAC \\ fs []
+  \\ pairarg_tac \\ fs []
+  \\ rw [] \\ fs []
+  \\ fs [cut_state_def] \\ rveq
+  \\ first_x_assum (qspec_then ‘dec_clock s1’ mp_tac)
+  \\ imp_res_tac evaluate_clock \\ fs [dec_clock_def]
+QED
+
+Theorem mark_all_syntax_ok:
+  ∀prog q b.
+     mark_all prog = (q,b) ==>
+     b = no_Loop q ∧ syntax_ok q
+Proof
+  recInduct mark_all_ind \\ rpt conj_tac
   \\ rpt gen_tac \\ strip_tac
-
-
-
-    \\ fs [every_prog_def,no_Loop_def,mark_all_def]
-  \\ rpt strip_tac \\ rveq \\ fs []
-  \\ fs [every_prog_def,no_Loop_def]
-  \\ fs [] \\ rpt (pairarg_tac \\ fs [])
-
-
+  THEN1
+   (fs [mark_all_def]
+    \\ rpt (pairarg_tac \\ fs []) \\ rveq
+    \\ IF_CASES_TAC
+    \\ fs [evaluate_def,every_prog_def,no_Loop_def,syntax_ok_def])
+  THEN1
+   (fs [mark_all_def]
+    \\ rpt (pairarg_tac \\ fs []) \\ rveq
+    \\ fs [every_prog_def,no_Loop_def,syntax_ok_def])
+  THEN1
+   (fs [mark_all_def]
+    \\ rpt (pairarg_tac \\ fs []) \\ rveq
+    \\ IF_CASES_TAC \\ fs []
+    \\ fs [no_Loop_def,every_prog_def,syntax_ok_def])
+  THEN1 fs [mark_all_def,syntax_ok_def]
+  THEN1
+   (fs [mark_all_def] \\ rveq
     \\ every_case_tac \\ fs []
-    \\ rpt strip_tac \\ rveq \\ fs []
-    \\ fs [] \\ rpt (pairarg_tac \\ fs [])
+    \\ fs [no_Loop_def,every_prog_def,syntax_ok_def]
+    \\ rpt (pairarg_tac \\ fs []) \\ rveq
+    \\ IF_CASES_TAC \\ fs []
+    \\ fs [every_prog_def,syntax_ok_def,no_Loop_def])
+  \\ fs [mark_all_def] \\ rveq
+  \\ fs [every_prog_def,no_Loop_def,syntax_ok_def]
+QED
+
+Theorem mark_all_evaluate:
+  ∀prog q b.
+     mark_all prog = (q,b) ==>
+     ∀s. evaluate (prog,s) = evaluate (q,s)
+Proof
+  recInduct mark_all_ind \\ rpt conj_tac
+  \\ rpt gen_tac \\ strip_tac
+  THEN1
+   (fs [mark_all_def]
+    \\ rpt (pairarg_tac \\ fs []) \\ rveq
+    \\ IF_CASES_TAC \\ fs [evaluate_def])
+  THEN1
+   (fs [mark_all_def]
+    \\ rpt (pairarg_tac \\ fs []) \\ rveq
+    \\ match_mp_tac evaluate_Loop_body_same \\ fs [])
+  THEN1
+   (fs [mark_all_def]
+    \\ rpt (pairarg_tac \\ fs []) \\ rveq
+    \\ IF_CASES_TAC \\ fs []
+    \\ fs [every_prog_def,evaluate_def]
+    \\ fs [no_Loop_def,every_prog_def]
+    \\ rw [] \\ every_case_tac \\ fs [])
+  THEN1 fs [mark_all_def,evaluate_def]
+  THEN1
+   (fs [mark_all_def] \\ rveq
     \\ every_case_tac \\ fs []
-    \\ fs [every_prog_def,no_Loop_def]
-    \\ rpt strip_tac \\ rveq \\ fs []
-    \\ fs [every_prog_def,no_Loop_def]
-
-
-
-    \\ pop_assum mp_tac
-  \\ once_rewrite_tac [mark_all_def]
-  \\ fs [] \\ rpt (pairarg_tac \\ fs [])
-  \\ rpt strip_tac \\ rveq \\ fs []
+    \\ fs [no_Loop_def,every_prog_def,evaluate_def]
+    \\ rpt (pairarg_tac \\ fs []) \\ rveq
+    \\ IF_CASES_TAC \\ fs []
+    \\ fs [every_prog_def,evaluate_def])
+  \\ fs [mark_all_def] \\ rveq
+  \\ simp [evaluate_def]
   \\ fs [every_prog_def,no_Loop_def]
+QED
 
-    \\ fs [CaseEq"bool"]
-    \\ rpt strip_tac \\ rveq \\ fs []
-    \\ fs [every_prog_def,no_Loop_def]
-    \\ cheat
+Definition SmartSeq_def:
+  SmartSeq p q = if p = Skip then q else
+                 if q = Skip then p else Seq p (q:'a wheatLang$prog)
+End
 
-    every_case_tac \\ fs []
-    \\ fs [] \\ rpt (pairarg_tac \\ fs [])
-    \\ fs [every_prog_def,no_Loop_def]
+Definition comp_no_loop_def:
+  (comp_no_loop p (Seq p1 p2) =
+    SmartSeq (comp_no_loop p p1) (comp_no_loop p p2)) /\
+  (comp_no_loop p (If x1 x2 x3 p1 p2 l1) =
+    If x1 x2 x3 (comp_no_loop p p1) (comp_no_loop p p2) l1) /\
+  (comp_no_loop p (Call ret dest args handler l) =
+    Call ret dest args (case handler of
+                        | SOME (n,q) => SOME (n,comp_no_loop p q)
+                        | NONE => NONE) l) /\
+  (comp_no_loop p Break = FST p) /\
+  (comp_no_loop p Continue = SND p) /\
+  (comp_no_loop p (Mark prog) = comp_no_loop p prog) /\
+  (comp_no_loop p prog = prog)
+End
 
+Definition store_cont_def:
+  store_cont live code (n,funs) =
+    let params = MAP FST (toSortedAList live) in
+    let funs = (n,params,code) :: funs in
+    let cont = Call NONE (SOME n) params NONE LN in
+      (cont:'a wheatLang$prog, (n+1,funs))
+End
 
-    Cases_on ‘t1’
-    \\ rpt strip_tac \\ rveq \\ fs []
-    \\ fs [every_prog_def,no_Loop_def]
+Definition comp_with_loop_def:
+  (comp_with_loop p (Seq p1 p2) cont s =
+     let (q2,s) = comp_with_loop p p2 cont s in
+       comp_with_loop p p1 q2 s) ∧
+  (comp_with_loop p (If x1 x2 x3 p1 p2 l1) cont s =
+     let (cont,s) = store_cont l1 cont s in
+     let (q1,s) = comp_with_loop p p1 cont s in
+     let (q2,s) = comp_with_loop p p2 cont s in
+       (If x1 x2 x3 q1 q2 LN,s)) /\
+  (comp_with_loop p (Call ret dest args handler l) cont s =
+     case handler of
+     | NONE => (SmartSeq (Call ret dest args NONE l) cont,s)
+     | SOME (n,q) =>
+         let (cont,s) = store_cont l cont s in
+         let (q,s) = comp_with_loop p q cont s in
+           (SmartSeq (Call ret dest args (SOME (n,q)) l) cont,s)) /\
+  (comp_with_loop p Break cont s = (FST p,s)) /\
+  (comp_with_loop p Continue cons s = (SND p,s)) /\
+  (comp_with_loop p (Mark prog) cont s = (SmartSeq (comp_no_loop p prog) cont,s)) /\
+  (comp_with_loop p (Loop live_in body live_out) cont s =
+     let (cont,s) = store_cont live_out cont s in
+     let params = MAP FST (toSortedAList live_in) in
+     let enter = Call NONE (SOME (FST s)) params NONE LN in
+     let (body,n,funs) = comp_with_loop (cont,enter) body Skip s in
+     let funs = (n,params,body) :: funs in
+       (enter,(n+1,funs))) ∧
+  (comp_with_loop p prog cont s = (Skip,s)) (* impossible case *)
+End
 
+Definition comp_def:
+  comp (name,params,prog) s =
+    let (body,n,funs) = comp_with_loop (Skip,Skip) prog Skip s in
+      (n,(name,params,body)::funs)
+End
 
+Definition comp_all_def:
+  comp_all code =
+    let n = FOLDR MAX 0 (MAP FST code) + 1 in
+      SND (FOLDR comp (n,[]) code)
+End
+
+Definition has_code_def:
+  has_code (n,funs) code =
+    EVERY (\(n,p,b). lookup n code = SOME (p,b)) funs
+End
+
+Definition state_rel_def:
+  state_rel s t <=>
+    ∃c. t = s with code := c ∧
+        ∀n params body.
+          lookup n s.code = SOME (params, body) ⇒
+          syntax_ok body ∧
+          ∃init. has_code (comp (n,params,body) init) t.code
+End
+
+val goal =
+  ``λ(prog, s). ∀res s1 t.
+    evaluate (prog,s) = (res,s1) ∧ state_rel s t ⇒
+    if syntax_ok prog then
+      ∀p result cont s q s'.
+        comp_with_loop p prog cont s = (q,s') ∧
+        has_code s' t.code ⇒
+        ∃ck t1.
+          evaluate (Seq q cont,t with clock := t.clock + ck) = result ⇒
+          state_rel s1 t1 ∧
+          case res of
+          | SOME Continue => result = evaluate (FST p,t1)
+          | SOME Break => result = evaluate (SND p,t1)
+          | _ => result = (res,t1)
+    else no_Loop prog ⇒
+      ∀p result.
+        ∃ck t1.
+          evaluate (comp_no_loop p prog,t with clock := t.clock + ck) = result ⇒
+          state_rel s1 t1 ∧
+          case res of
+          | SOME Continue => result = evaluate (FST p,t1)
+          | SOME Break => result = evaluate (SND p,t1)
+          | _ => result = (res,t1)``
+
+local
+  val ind_thm = wheatSemTheory.evaluate_ind
+    |> ISPEC goal
+    |> CONV_RULE (DEPTH_CONV PairRules.PBETA_CONV) |> REWRITE_RULE [];
+  fun list_dest_conj tm = if not (is_conj tm) then [tm] else let
+    val (c1,c2) = dest_conj tm in list_dest_conj c1 @ list_dest_conj c2 end
+  val ind_goals = ind_thm |> concl |> dest_imp |> fst |> list_dest_conj
+in
+  fun get_goal s = first (can (find_term (can (match_term (Term [QUOTE s]))))) ind_goals
+  fun compile_correct_tm () = ind_thm |> concl |> rand
+  fun the_ind_thm () = ind_thm
+end
+
+Theorem compile_Skip:
+  ^(get_goal "wheatLang$Skip")
+Proof
+  cheat
+QED
+
+Theorem compile_Continue:
+  ^(get_goal "wheatLang$Continue") ∧
+  ^(get_goal "wheatLang$Break")
+Proof
+  cheat
+QED
+
+Theorem compile_Mark:
+  ^(get_goal "wheatLang$Mark") ∧
+  ^(get_goal "wheatLang$Tick")
+Proof
+  cheat
+QED
+
+Theorem compile_Return:
+  ^(get_goal "wheatLang$Return") ∧
+  ^(get_goal "wheatLang$Raise")
+Proof
+  cheat
+QED
+
+Theorem compile_Assign:
+  ^(get_goal "wheatLang$Assign") ∧
+  ^(get_goal "wheatLang$LocValue")
+Proof
+  cheat
+QED
+
+Theorem compile_Store:
+  ^(get_goal "wheatLang$Store") ∧
+  ^(get_goal "wheatLang$LoadByte")
+Proof
+  cheat
+QED
+
+Theorem compile_StoreGlob:
+  ^(get_goal "wheatLang$StoreGlob") ∧
+  ^(get_goal "wheatLang$LoadGlob")
+Proof
+  cheat
+QED
+
+Theorem compile_Loop:
+  ^(get_goal "wheatLang$Loop")
+Proof
+  cheat
+QED
+
+Theorem compile_Call:
+  ^(get_goal "syntax_ok (wheatLang$Call _ _ _ _ _)")
+Proof
+  cheat
+QED
+
+Theorem compile_Seq:
+  ^(get_goal "syntax_ok (wheatLang$Seq _ _)")
+Proof
+  cheat
+QED
+
+Theorem compile_If:
+  ^(get_goal "wheatLang$If")
+Proof
+  cheat
+QED
+
+Theorem compile_FFI:
+  ^(get_goal "wheatLang$FFI")
+Proof
+  cheat
+QED
+
+Theorem compile_correct:
+  ^(compile_correct_tm())
+Proof
+  match_mp_tac (the_ind_thm())
+  \\ EVERY (map strip_assume_tac [compile_Skip, compile_Continue,
+       compile_Mark, compile_Return, compile_Assign, compile_Store,
+       compile_StoreGlob, compile_Call, compile_Seq, compile_If,
+       compile_FFI, compile_Loop])
+  \\ asm_rewrite_tac [] \\ rw [] \\ rpt (pop_assum kall_tac)
+QED
 
 val _ = export_theory();
